src/main/translation/structure/type.scala
@@ -8,6 +8,7 @@ case object TypeChar extends Type
 case object TypeNat extends Type
 case class SeqType(elementType: Type) extends Type
 case class SetType(elementType: Type) extends Type
-case class NamedType(name: String, generics: Option[List[Type]]) extends Type
+case class CreatedType(name: String, generics: List[Type]) extends Type
+case class GenericType(name: String) extends Type
 case class TupleType(elements: List[Type]) extends Type
 case class ArrowType(from: Type, to: Type) extends Type
