src/main/translation/translation.scala
@@ -3,5 +3,6 @@ package translation.translation
 import translation.structure.*
 
 case class Context(
-    functionData: Map[String, List[Parameter]]
+    functionData: Map[String, List[String]],
+    typeData: Map[String, String]
 )
