src/test/output/unfoldingSorted.dfy
@@ -1,23 +1,31 @@
-datatype Option<T> = None | Some(value: T)
+datatype Option<A> = None | Some(value: A)
 
-datatype List<T> = Nil | Cons(head: T, tail: List<T>)
+datatype List<A> = Nil | Cons(head: A, tail: List<A>)
 
-function unfoldingSortedM<S, T>(start: S, next: S -> Option<(S, T)>, leq: (T, T) -> bool, max: int): List<T>
+function unfoldingSortedM<A, B>(start: A, next: A -> Option<(A, B)>, leq: (B, B) -> bool, max: int): List<B>
 {loopM(start, next, leq, max, Nil)}
 
-function unfoldingSorted5<State, Elem>(start: State, next: State -> Option<(State, Elem)>, leq: (Elem, Elem) -> bool, max: int): List<Elem>
+function unfoldingSorted5<A, B>(start: A, next: A -> Option<(A, B)>, leq: (B, B) -> bool, max: int): List<B>
 {go5(start, next, leq, Nil, max)}
 
-function unfoldingSorted4<State, Elem>(start: State, next: State -> Option<(State, Elem)>, leq: (Elem, Elem) -> bool, max: int): List<Elem>
+function unfoldingSorted4<A, B>(start: A, next: A -> Option<(A, B)>, leq: (B, B) -> bool, max: int): List<B>
 {go4(start, next, leq, Nil, max)}
 
-function unfoldingSorted3<State, Elem>(start: State, next: State -> Option<(State, Elem)>, leq: (Elem, Elem) -> bool, max: int): List<Elem>
+function unfoldingSorted3<A, B>(start: A, next: A -> Option<(A, B)>, leq: (B, B) -> bool, max: int): List<B>
 {go3(start, next, Nil, max)}
 
-function unfoldingSorted1<State, Elem>(start: State, next: State -> Option<(State, Elem)>, leq: (Elem, Elem) -> bool, max: int): List<Elem>
+function unfoldingSorted1<A, B>(start: A, next: A -> Option<(A, B)>, leq: (B, B) -> bool, max: int): List<B>
 {go1(start, next, leq, Nil, max)}
 
-function go5<State, Elem>(s: State, next: State -> Option<(State, Elem)>, leq: (Elem, Elem) -> bool, xs: List<Elem>, fuel: int): List<Elem>
+function go1<A, B>(s: A, next: A -> Option<(A, B)>, leq: (B, B) -> bool, xs: List<B>, fuel: int): List<B>
+decreases (if (fuel <= 0) then 0 else fuel)
+{if (fuel <= 0) then xs else match next(s) {
+case Some((nxtS, t)) => go1(nxtS, next, leq, insertSorted1(t, leq, xs), fuel - 1)
+case None => xs
+}
+}
+
+function go5<A, B>(s: A, next: A -> Option<(A, B)>, leq: (B, B) -> bool, xs: List<B>, fuel: int): List<B>
 decreases (if (fuel <= 0) then 0 else fuel)
 {if (fuel <= 0) then xs else match next(s) {
 case Some((nxtS, t)) => go5(nxtS, next, leq, insertSorted5(t, leq, xs), fuel - 1)
@@ -25,7 +33,23 @@ case None => xs
 }
 }
 
-function insertSorted5<Elem>(t: Elem, leq: (Elem, Elem) -> bool, xs: List<Elem>): List<Elem>
+function insertM<A>(xs: List<A>, leq: (A, A) -> bool, t: A): List<A>
+decreases (xs)
+{match xs {
+case Nil => Cons(t, Nil)
+case Cons(hd, tl) => if (leq(t, hd)) then Cons(t, xs) else Cons(hd, insertM(tl, leq, t))
+}
+}
+
+function loopM<A, B>(s: A, next: A -> Option<(A, B)>, leq: (B, B) -> bool, fuel: int, xs: List<B>): List<B>
+decreases (if (fuel <= 0) then 0 else fuel)
+{if (fuel <= 0) then xs else match next(s) {
+case Some((nxtS, t)) => loopM(nxtS, next, leq, fuel - 1, insertM(xs, leq, t))
+case None => xs
+}
+}
+
+function insertSorted5<A>(t: A, leq: (A, A) -> bool, xs: List<A>): List<A>
 decreases (xs)
 {match xs {
 case Nil => Cons(t, Nil)
@@ -33,7 +57,15 @@ case Cons(hd, tl) => if (leq(t, hd)) then Cons(t, xs) else Cons(hd, insertSorted
 }
 }
 
-function go4<State, Elem>(s: State, next: State -> Option<(State, Elem)>, leq: (Elem, Elem) -> bool, xs: List<Elem>, fuel: int): List<Elem>
+function go3<A, B>(s: A, next: A -> Option<(A, B)>, xs: List<B>, fuel: int): List<B>
+decreases (if (fuel <= 0) then 0 else fuel)
+{if (fuel <= 0) then xs else match next(s) {
+case Some((nxtS, t)) => go3(nxtS, next, insertSorted3(t, xs), fuel - 1)
+case None => xs
+}
+}
+
+function go4<A, B>(s: A, next: A -> Option<(A, B)>, leq: (B, B) -> bool, xs: List<B>, fuel: int): List<B>
 decreases (if (fuel <= 0) then 0 else fuel)
 {if (fuel <= 0) then xs else match next(s) {
 case Some((nxtS, t)) => go4(nxtS, next, leq, insertSorted4(t, leq, xs), fuel - 1)
@@ -45,23 +77,7 @@ case Nil => xs
 }
 }
 
-function insertSorted4<Elem>(t: Elem, leq: (Elem, Elem) -> bool, xs: List<Elem>): List<Elem>
-decreases (xs)
-{match xs {
-case Nil => Cons(t, Nil)
-case Cons(hd, tl) => if (leq(t, hd)) then Cons(t, xs) else Cons(hd, insertSorted4(t, leq, tl))
-}
-}
-
-function go3<State, Elem>(s: State, next: State -> Option<(State, Elem)>, xs: List<Elem>, fuel: int): List<Elem>
-decreases (if (fuel <= 0) then 0 else fuel)
-{if (fuel <= 0) then xs else match next(s) {
-case Some((nxtS, t)) => go3(nxtS, next, insertSorted3(t, xs), fuel - 1)
-case None => xs
-}
-}
-
-function insertSorted3<Elem>(t: Elem, xs: List<Elem>): List<Elem>
+function insertSorted3<A>(t: A, xs: List<A>): List<A>
 decreases (xs)
 {match xs {
 case Nil => Cons(t, Nil)
@@ -69,15 +85,15 @@ case Cons(hd, tl) => Cons(hd, insertSorted3(t, tl))
 }
 }
 
-function go1<State, Elem>(s: State, next: State -> Option<(State, Elem)>, leq: (Elem, Elem) -> bool, xs: List<Elem>, fuel: int): List<Elem>
-decreases (if (fuel <= 0) then 0 else fuel)
-{if (fuel <= 0) then xs else match next(s) {
-case Some((nxtS, t)) => go1(nxtS, next, leq, insertSorted1(t, leq, xs), fuel - 1)
-case None => xs
+function insertSorted4<A>(t: A, leq: (A, A) -> bool, xs: List<A>): List<A>
+decreases (xs)
+{match xs {
+case Nil => Cons(t, Nil)
+case Cons(hd, tl) => if (leq(t, hd)) then Cons(t, xs) else Cons(hd, insertSorted4(t, leq, tl))
 }
 }
 
-function insertSorted1<Elem>(t: Elem, leq: (Elem, Elem) -> bool, xs: List<Elem>): List<Elem>
+function insertSorted1<A>(t: A, leq: (A, A) -> bool, xs: List<A>): List<A>
 decreases (xs)
 {match xs {
 case Nil => Cons(t, Nil)
@@ -85,55 +101,34 @@ case Cons(hd, tl) => if (leq(t, hd)) then Cons(t, xs) else Cons(hd, insertSorted
 }
 }
 
-function loopM<S, T>(s: S, next: S -> Option<(S, T)>, leq: (T, T) -> bool, fuel: int, xs: List<T>): List<T>
-decreases (if (fuel <= 0) then 0 else fuel)
-{if (fuel <= 0) then xs else match next(s) {
-case Some((nxtS, t)) => loopM(nxtS, next, leq, fuel - 1, insertM(xs, leq, t))
-case None => xs
-}
-}
-
-function insertM<T>(xs: List<T>, leq: (T, T) -> bool, t: T): List<T>
-decreases (xs)
-{match xs {
-case Nil => Cons(t, Nil)
-case Cons(hd, tl) => if (leq(t, hd)) then Cons(t, xs) else Cons(hd, insertM(tl, leq, t))
-}
-}
-
-lemma unfoldingSortedM_unfoldingSorted5_Equivalence<S, T>(start: S, next: S -> Option<(S, T)>, leq: (T, T) -> bool, max: int)
+lemma unfoldingSortedM_unfoldingSorted5_Equivalence<A, B>(start: A, next: A -> Option<(A, B)>, leq: (B, B) -> bool, max: int)
 ensures unfoldingSortedM(start, next, leq, max) == unfoldingSorted5(start, next, leq, max)
 {{loopM_go5_Equivalence(start, next, leq, max, Nil);}}
 
-lemma unfoldingSortedM_unfoldingSorted4_Equivalence<S, T>(start: S, next: S -> Option<(S, T)>, leq: (T, T) -> bool, max: int)
+lemma unfoldingSortedM_unfoldingSorted4_Equivalence<A, B>(start: A, next: A -> Option<(A, B)>, leq: (B, B) -> bool, max: int)
 ensures unfoldingSortedM(start, next, leq, max) == unfoldingSorted4(start, next, leq, max)
 {{loopM_go4_Equivalence(start, next, leq, max, Nil);}}
 
-lemma unfoldingSortedM_unfoldingSorted3_Equivalence<S, T>(start: S, next: S -> Option<(S, T)>, leq: (T, T) -> bool, max: int)
+lemma unfoldingSortedM_unfoldingSorted3_Equivalence<A, B>(start: A, next: A -> Option<(A, B)>, leq: (B, B) -> bool, max: int)
 ensures unfoldingSortedM(start, next, leq, max) == unfoldingSorted3(start, next, leq, max)
-{{loopM_go3_Equivalence(start, next, leq, max, Nil);}}
+{{}}
 
-lemma unfoldingSortedM_unfoldingSorted1_Equivalence<S, T>(start: S, next: S -> Option<(S, T)>, leq: (T, T) -> bool, max: int)
+lemma unfoldingSortedM_unfoldingSorted1_Equivalence<A, B>(start: A, next: A -> Option<(A, B)>, leq: (B, B) -> bool, max: int)
 ensures unfoldingSortedM(start, next, leq, max) == unfoldingSorted1(start, next, leq, max)
 {{loopM_go1_Equivalence(start, next, leq, max, Nil);}}
 
-lemma loopM_go5_Equivalence<S, T>(s: S, next: S -> Option<(S, T)>, leq: (T, T) -> bool, fuel: int, xs: List<T>)
+lemma loopM_go5_Equivalence<A, B>(s: A, next: A -> Option<(A, B)>, leq: (B, B) -> bool, fuel: int, xs: List<B>)
 decreases (if (fuel <= 0) then 0 else fuel)
-ensures loopM(s, next, leq, fuel, xs) == go5(s, next, leq, fuel, xs)
+ensures loopM(s, next, leq, fuel, xs) == go5(s, next, leq, xs, fuel)
 {{}}
 
-lemma loopM_go4_Equivalence<S, T>(s: S, next: S -> Option<(S, T)>, leq: (T, T) -> bool, fuel: int, xs: List<T>)
+lemma loopM_go4_Equivalence<A, B>(s: A, next: A -> Option<(A, B)>, leq: (B, B) -> bool, fuel: int, xs: List<B>)
 decreases (if (fuel <= 0) then 0 else fuel)
-ensures loopM(s, next, leq, fuel, xs) == go4(s, next, leq, fuel, xs)
+ensures loopM(s, next, leq, fuel, xs) == go4(s, next, leq, xs, fuel)
 {{}}
 
-lemma loopM_go3_Equivalence<S, T>(s: S, next: S -> Option<(S, T)>, leq: (T, T) -> bool, fuel: int, xs: List<T>)
+lemma loopM_go1_Equivalence<A, B>(s: A, next: A -> Option<(A, B)>, leq: (B, B) -> bool, fuel: int, xs: List<B>)
 decreases (if (fuel <= 0) then 0 else fuel)
-ensures loopM(s, next, leq, fuel, xs) == go3(s, next, leq, fuel, xs)
-{{}}
-
-lemma loopM_go1_Equivalence<S, T>(s: S, next: S -> Option<(S, T)>, leq: (T, T) -> bool, fuel: int, xs: List<T>)
-decreases (if (fuel <= 0) then 0 else fuel)
-ensures loopM(s, next, leq, fuel, xs) == go1(s, next, leq, fuel, xs)
+ensures loopM(s, next, leq, fuel, xs) == go1(s, next, leq, xs, fuel)
 {{}}
 
